

ϵ - δ definition: $\forall \epsilon > 0, \exists \delta > 0$, such that $|x - x_0| < \delta \Rightarrow |f(x) - A| < \epsilon$

$$\lim_{x \rightarrow x_0} f(x) = A \quad \lim_{x \rightarrow +\infty} f(x) = A \quad \lim_{x \rightarrow -\infty} f(x) = A \quad \lim_{|x| \rightarrow +\infty} f(x) = A$$

$$\lim_{x \rightarrow x_0^-} f(x) = A \quad \lim_{x \rightarrow x_0^+} f(x) = A$$

Properties of limits

① Uniqueness $\lim_{x \rightarrow x_0} f(x) = a \quad \lim_{x \rightarrow x_0} f(x) = b \Leftrightarrow a = b$

② Boundedness $\lim_{x \rightarrow x_0} f(x)$ exists $\Rightarrow |f(x)| < M \quad \forall x \in (x_0 - \delta, x_0) \cup (x_0, x_0 + \delta)$

③ 保号性 $\lim_{x \rightarrow x_0} f(x) = A > 0 \Rightarrow \forall x \in (x_0 - \delta, x_0) \cup (x_0, x_0 + \delta) \quad f(x) > 0$

④ 保不等式性 $\lim_{x \rightarrow x_0} f(x)$ and $\lim_{x \rightarrow x_0} g(x)$ exists,
and $f(x) \leq g(x) \quad \forall x \in (x_0 - \delta, x_0) \cup (x_0, x_0 + \delta) \Rightarrow \lim_{x \rightarrow x_0} f(x) \leq \lim_{x \rightarrow x_0} g(x)$

⑤ Sandwich Theorem: $f(x) \leq h(x) \leq g(x) \quad \forall x \in (x_0 - \delta, x_0) \cup (x_0, x_0 + \delta)$ and
 $\lim_{x \rightarrow x_0} f(x) = \lim_{x \rightarrow x_0} g(x) = A \Rightarrow \lim_{x \rightarrow x_0} h(x) = A$

⑥ Arithmetic operations $+, -, \times, \div$

⑦ $\lim_{y \rightarrow y_0} f(y) = A \quad \lim_{x \rightarrow x_0} g(x) = y_0 \Rightarrow \lim_{x \rightarrow x_0} f(g(x)) = A$

Thm (Heine's theorem) $\lim_{x \rightarrow x_0} f(x) = A \Leftrightarrow \lim_{n \rightarrow \infty} f(x_n) = A \quad \forall \{x_n\} \rightarrow x_0$

Infinitesimal quantity : $\lim_{x \rightarrow x_0} f(x) = 0$

① higher order : $\lim_{x \rightarrow x_0} f(x) = 0$ $\lim_{x \rightarrow x_0} g(x) = 0$, $f(x)$ higher order than $g(x)$

$$\lim_{x \rightarrow x_0} \frac{f(x)}{g(x)} = 0$$

② Same order : $\lim_{x \rightarrow x_0} f(x) = 0$ $\lim_{x \rightarrow x_0} g(x) = 0$, $\Rightarrow \lim_{x \rightarrow x_0} \frac{f(x)}{g(x)} = c \neq 0$

③ Equivalent : $\lim_{x \rightarrow x_0} f(x) = 0$ $\lim_{x \rightarrow x_0} g(x) = 0$, $\Rightarrow \lim_{x \rightarrow x_0} \frac{f(x)}{g(x)} = 1$

Infinite quantity (无穷大)

Defn : If f is well-defined on $(x_0 - \varepsilon, x_0) \cup (x_0, x_0 + \varepsilon)$, and

$$\lim_{x \rightarrow x_0} |f(x)| = +\infty$$

then we say f is an infinite quantity as $x \rightarrow x_0$.

$$\text{E.g.: } \lim_{x \rightarrow 0} \frac{1}{x^2} = +\infty \quad \lim_{x \rightarrow 0^-} \frac{1}{x} = -\infty \quad \lim_{x \rightarrow 0^+} \frac{1}{x} = +\infty \quad \lim_{x \rightarrow 0} \left| \frac{1}{x} \right| = \infty$$

Properties : If $\lim_{x \rightarrow x_0} f(x) = +\infty$ $\lim_{x \rightarrow x_0} g(x) = +\infty$ $\lim_{x \rightarrow x_0} h(x) = A \neq 0$ $|A| < +\infty$

then we have

$$\textcircled{1} \lim_{x \rightarrow x_0} (f(x) + g(x)) = +\infty \quad \lim_{x \rightarrow x_0} (f(x) + h(x)) = +\infty$$

$$\textcircled{2} \lim_{x \rightarrow x_0} f(x) \cdot g(x) = +\infty \quad \lim_{x \rightarrow x_0} f(x) \cdot h(x) = +\infty.$$

Commonly used equivalent infinitesimal quantity.

$$\lim_{x \rightarrow x_0} \frac{f(x)}{g(x)} = 1 \rightarrow f(x) \sim g(x) \text{ at } x_0$$

① At $x_0 = 0$ $\sin x \sim x$ $\arcsin x \sim x$

$\tan x \sim x$ $\arctan x \sim x$

$\ln(x+1) \sim x$ $e^x - 1 \sim x$

$a^x - 1 \sim x \ln a$

$1 - \cos x \sim \frac{1}{2} x^2$

$\sqrt[n]{1+x} - 1 \sim \frac{1}{n} x$

② At $x_0 = 1$ $\ln x \sim x - 1$

E.g. ① $\lim_{x \rightarrow 0} \frac{\arctan x}{\sin 4x} = \lim_{x \rightarrow 0} \frac{x}{4x} = \frac{1}{4}$ $\arctan x \sim x$ $\sin x \sim x$

② $\lim_{x \rightarrow 0} \frac{\tan x - \sin x}{\sin(x^3)} = \lim_{x \rightarrow 0} \frac{\frac{\sin x}{\cos x} - \sin x}{\sin(x^3)} = \lim_{x \rightarrow 0} \frac{\sin x}{\cos x} \frac{(1 - \cos x)}{\sin x^3}$

$= \lim_{x \rightarrow 0} \frac{1}{\cos x} \frac{x \cdot \frac{1}{2} x^2}{x^3} = \frac{1}{2}$

E.g.: ① $\lim_{x \rightarrow \frac{\pi}{2}} 2(\sin x - \cos x - x^2) = 2 - \frac{\pi^2}{2}$

② $\lim_{x \rightarrow 0} \frac{x^2 - 1}{2x^2 - x - 1} = 1$

③ $\lim_{x \rightarrow 1} \frac{x^2 - 1}{2x^2 - x - 1} = \lim_{x \rightarrow 1} \frac{(x+1)(x-1)}{(x-1)(2x+1)} = \lim_{x \rightarrow 1} \frac{x+1}{2x+1} = \frac{2}{3}$

④ $\lim_{x \rightarrow 0} \frac{(x-1)^3 + (1-3x)}{x^2 + 2x^3} = \lim_{x \rightarrow 0} \frac{x^3 - 3x^2 + 3x - 1 + 1 - 3x}{x^2 + 2x^3} = \lim_{x \rightarrow 0} \frac{x^2(x-3)}{x^2(1+2x)} = -3$

$$\textcircled{5} \lim_{x \rightarrow 4} \frac{\sqrt{1+2x} - 3}{\sqrt{x} - 2} = \lim_{x \rightarrow 4} \frac{(\sqrt{1+2x} - 3)(\sqrt{1+2x} + 3)}{(\sqrt{x} - 2)(\sqrt{1+2x} + 3)} = \lim_{x \rightarrow 4} \frac{(1+2x-9)}{(\sqrt{x}-2)(\sqrt{1+2x}+3)}$$

$$= \lim_{x \rightarrow 4} \frac{2(x-4)(\sqrt{1+2x})}{(\sqrt{x}-2)(\sqrt{1+2x}+3)} = \lim_{x \rightarrow 4} \frac{2(x-4)}{(\sqrt{x}-2)(\sqrt{1+2x}+3)} = \frac{4}{5}$$

$$\textcircled{6} \lim_{x \rightarrow 0} \frac{\sqrt{a^2+x} - a}{x} \quad (a > 0) = \lim_{x \rightarrow 0} \frac{(\sqrt{a^2+x} - a)(\sqrt{a^2+x} + a)}{x(\sqrt{a^2+x} + a)} = \lim_{x \rightarrow 0} \frac{x}{x(\sqrt{a^2+x} + a)} = \frac{1}{2a}$$

$$\textcircled{7} \lim_{x \rightarrow 1} \frac{x^n - 1}{x^m - 1} = \lim_{x \rightarrow 1} \frac{(x-1)(x^{n-1} + x^{n-2} + \dots + x + 1)}{(x-1)(x^{m-1} + x^{m-2} + \dots + x + 1)} = \frac{n}{m}$$

2. Find the limits by using squeeze theorem.

$$\textcircled{1} \lim_{x \rightarrow \infty} \frac{x - \cos x}{x} = \lim_{x \rightarrow \infty} 1 - \frac{\cos x}{x} = 1 \quad 1 - \frac{1}{x} \leq 1 - \frac{\cos x}{x} \leq 1 + \frac{1}{x}$$

$$\textcircled{2} \lim_{x \rightarrow \infty} \frac{x \cdot \sin x}{x^2 - 4} = 0 \quad \frac{-x}{x^2 - 4} \leq \frac{x \sin x}{x^2 - 4} \leq \frac{x}{x^2 - 4}$$

$$\textcircled{3} \lim_{x \rightarrow \infty} \frac{[x]}{x} = 1 \quad x-1 \leq [x] \leq x+1$$

3. Based on $\lim_{x \rightarrow 0} \frac{\sin x}{x} = 1$, find the following limits.

$$\textcircled{1} \lim_{x \rightarrow 0} \frac{\sin 2x}{x} = \lim_{x \rightarrow 0} 2 \frac{\sin 2x}{2x} = 2$$

$$\textcircled{2} \lim_{x \rightarrow 0} \frac{\sin x^3}{\sin^2 x} = \lim_{x \rightarrow 0} \frac{x^2}{\sin^2 x} \frac{\sin x^3}{x^3} \cdot x = 0$$

$$\textcircled{3} \lim_{x \rightarrow 0} \frac{\tan x}{x} = \frac{\sin x}{x} \cdot \frac{1}{\cos x} = 1$$

$$\textcircled{4} \lim_{x \rightarrow \frac{\pi}{2}} \frac{\cos x}{x - \frac{\pi}{2}} \quad \text{let } y = x - \frac{\pi}{2} \quad y \rightarrow 0 \text{ as } x \rightarrow \frac{\pi}{2} \quad x = y + \frac{\pi}{2}$$

$$= \lim_{y \rightarrow 0} \frac{\cos(y + \frac{\pi}{2})}{y} = \lim_{y \rightarrow 0} \frac{-\sin y}{y} = -1$$

$$\textcircled{5} \lim_{x \rightarrow 0} \frac{\tan x - \sin x}{x^3} = \lim_{x \rightarrow 0} \frac{\sin x - \sin x \cos x}{x^3 \cos x} = \lim_{x \rightarrow 0} \frac{\sin x}{x} \frac{1 - \cos x}{x^2} \frac{1}{\cos x} = \frac{1}{2}$$

$$\sin x^3 = \sin(x^3)$$

$$\sin^2 x = (\sin x)^2$$

$$\textcircled{6} \lim_{x \rightarrow 0} \frac{\arctan x}{x} \quad \text{let } y = \arctan x \text{ then } x = \tan y \quad y \rightarrow 0 \text{ as } x \rightarrow 0$$

$$= \lim_{y \rightarrow 0} \frac{y}{\tan y} = 1$$

$$\textcircled{7} \lim_{x \rightarrow +\infty} x \sin \frac{1}{x} = 1 \quad \text{let } y = \frac{1}{x} \text{ then } x = \frac{1}{y} \quad y \rightarrow 0 \text{ as } x \rightarrow +\infty$$

$$\textcircled{8} \lim_{x \rightarrow a} \frac{\sin^2 x - \sin^2 a}{x - a}$$

$$\sin a + \sin b = 2 \sin \left(\frac{a+b}{2} \right) \cos \left(\frac{a-b}{2} \right)$$

$$\sin a - \sin b = 2 \cos \left(\frac{a+b}{2} \right) \sin \left(\frac{a-b}{2} \right)$$

$$\sin 2a = 2 \sin a \cdot \cos a$$

$$= \lim_{x \rightarrow a} \frac{(\sin x + \sin a)(\sin x - \sin a)}{x - a}$$

$$= \lim_{x \rightarrow a} \frac{2 \sin \left(\frac{x+a}{2} \right) \cos \left(\frac{x-a}{2} \right) \cdot 2 \sin \left(\frac{x-a}{2} \right) \cos \left(\frac{x+a}{2} \right)}{x - a}$$

$$= \lim_{x \rightarrow a} \frac{2 \sin \left(\frac{x+a}{2} \right) \cos \left(\frac{x+a}{2} \right) \cdot 2 \sin \left(\frac{x-a}{2} \right) \cos \left(\frac{x-a}{2} \right)}{x - a}$$

$$= \lim_{x \rightarrow a} \frac{\sin(x+a) \sin(x-a)}{x-a} = \lim_{x \rightarrow a} \sin(x+a) = \sin 2a$$

$$\lim_{x \rightarrow 0} (1+x)^{\frac{1}{x}} = e$$

4. Based on $\lim_{x \rightarrow \infty} \left(1 + \frac{1}{x}\right)^x = e$, find the following limits.

$$\textcircled{1} \lim_{x \rightarrow 0} (1+2x)^{\frac{1}{x}} = \lim_{x \rightarrow 0} (1+2x)^{\frac{1}{2x} \cdot 2} = \lim_{x \rightarrow 0} \left[(1+2x)^{\frac{1}{2x}} \right]^2 = e^2$$

$$\textcircled{2} \lim_{x \rightarrow 0} (1+\alpha x)^{\frac{1}{x}} \quad (\alpha > 0) = e^\alpha$$

$$\textcircled{3} \lim_{x \rightarrow 0} (1+\tan x)^{\cot x} \quad \text{let } y = \cot x \text{ then } \tan x = \frac{1}{y}.$$

$$|y| \rightarrow +\infty \text{ as } x \rightarrow 0$$

$$= \lim_{|y| \rightarrow +\infty} \left(1 + \frac{1}{y}\right)^y = e$$

$$\textcircled{4} \lim_{x \rightarrow 0} \left(\frac{1+x}{1-x} \right)^{\frac{1}{x}} = \lim_{x \rightarrow 0} \left(\frac{1-x+2x}{1-x} \right)^{\frac{1}{x}} = \lim_{x \rightarrow 0} \left(1 + \frac{2x}{1-x} \right)^{\frac{1}{x}}$$

$$\text{let } y = \frac{1-x}{2x} \quad x = \frac{1}{2y+1} \quad |y| \rightarrow +\infty \text{ as } x \rightarrow 0$$

$$= \lim_{|y| \rightarrow +\infty} \left(1 + \frac{1}{y}\right)^{2y+1} = \lim_{|y| \rightarrow +\infty} \left[\left(1 + \frac{1}{y}\right)^y \right]^2 \left(1 + \frac{1}{y}\right) = e^2 \cdot 1$$

$$\textcircled{5} \lim_{x \rightarrow +\infty} \left(\frac{3x+2}{3x-1} \right)^{2x-1} = \lim_{x \rightarrow +\infty} \left(1 + \frac{1}{x-\frac{1}{3}} \right)^{2x-1} \quad \text{let } y = x - \frac{1}{3}$$

$$= \lim_{y \rightarrow +\infty} \left(1 + \frac{1}{y} \right)^{2y-\frac{1}{3}} = e^2 \cdot 1$$

$$\textcircled{6} \lim_{x \rightarrow \infty} \left(1 + \frac{\alpha}{x} \right)^{\beta x} \quad \text{let } y = \frac{1}{x} \quad \text{then } x \rightarrow 0$$

$$= \lim_{x \rightarrow \infty} \left(1 + \frac{1}{y} \right)^{\beta \alpha y} = e^{\alpha \beta}$$

5. Using the equivalent infinitesimal quantity to find the limits.

$$\textcircled{1} \lim_{x \rightarrow 0} \frac{x \arctan \frac{1}{x}}{x - \cos x} = \lim_{x \rightarrow 0} \frac{1}{x - \cos x} = 0$$

$$\textcircled{2} \lim_{x \rightarrow 0} \frac{\sqrt{1+x^2} - 1}{1 - \cos x} = \lim_{x \rightarrow 0} \frac{\sqrt{1+x^2} - 1}{\frac{1}{2}x^2} \cdot \frac{\frac{1}{2}x^2}{1 - \cos x} = \lim_{x \rightarrow 0} \frac{(\sqrt{1+x^2} - 1)(\sqrt{1+x^2} + 1)}{\frac{1}{2}x^2(\sqrt{1+x^2} + 1)}$$

$$= \lim_{x \rightarrow 0} \frac{1+x^2-1}{\frac{1}{2}x^2(\sqrt{1+x^2}+1)} = \lim_{x \rightarrow 0} \frac{1}{\frac{1}{2}(\sqrt{1+x^2}+1)} = 1$$

$$\sin x \sim x \quad \arcsin x \sim x$$

$$\tan x \sim x \quad \arctan x \sim x$$

$$1 - \cos x \sim \frac{1}{2}x^2$$

$$\sqrt[n]{1+x} - 1 \sim \frac{1}{n}x$$

$$\ln(x+1) \sim x \quad e^x - 1 \sim x$$

$$a^x - 1 \sim x \ln a$$